(2\mu_1 +\mu_3)\pi(2, 0, 1, 0) =\lambda_1\pi(1, 0, 1, 0) + \lambda_3\pi(2, 0, 0, 0)
(\lambda_1 +\mu_1 +\mu_3)\pi(1, 0, 1, 0) = 2\mu_1\pi(2, 0, 1, 0) +\lambda_1\pi(0, 0, 1, 0) +\mu_3\pi(1, 0, 0, 0)
(\lambda_1 +\lambda_2 +\mu_3)\pi(0, 0, 1, 0) =\mu_1\pi(1, 0, 1, 0) +\lambda_3\pi(0, 0, 0, 0) +\mu_2\pi(0, 1, 1, 0)
(\mu_2 +\mu_3)\pi(0, 1, 1, 0) =\lambda_2\pi(0, 0, 1, 0) +\lambda_3\pi(0, 1, 0, 0)
(\mu_4 +\lambda_1)\pi(0, 0, 0, 1) =\lambda_4\pi(0, 0, 0, 0) +\mu_1\pi(1, 0, 0, 1)
(\lambda_1 +\lambda_2 +\lambda_3 +\lambda_4)\pi(0, 0, 0, 0) =\mu_3\pi(1, 0, 1, 0) +\mu_4\pi(0, 0, 0, 1) +\mu_1\pi(1, 0, 0, 0) +\mu_2\pi(0, 1, 0, 0)
(\mu_2 +\lambda_1 +\lambda_2 +\lambda_3)\pi(0, 1, 0, 0) =\lambda_2\pi(0, 0, 0, 0) +\mu_1\pi(1, 1, 0, 0)+2\mu_2\pi(0, 2, 0, 0) +\mu_3\pi(0, 1, 1, 0)
(2\mu_2 +\lambda_1)\pi(0, 2, 0, 0) =\lambda_2\pi(0, 1, 0, 0) +\mu_1\pi(1, 2, 0, 0)
(\mu_1 +\mu_4)\pi(1, 0, 0, 1) =\lambda_1\pi(0, 0, 0, 1) +\lambda_4\pi(1, 0, 0, 0)
(\lambda_4 +\lambda_1 +\mu_2 +\mu_1 +\lambda_3)\pi(1, 0, 0, 0) =\mu_4\pi(1, 0, 0, 1)+2\mu_1\pi(2, 0, 0, 0) +\mu_2\pi(1, 1, 0, 0) +\lambda_1\pi(0, 0, 0, 0) +\mu_3\pi(1, 0, 1, 0)
(\mu_2 +\lambda_1 +\lambda_2 +\mu_1)\pi(1, 1, 0, 0) =\lambda_2\pi(1, 0, 0, 0)+2\mu_1\pi(2, 1, 0, 0)+2\mu_2\pi(1, 2, 0, 0) +\lambda_1\pi(0, 1, 0, 0)
(2\mu_2 +\mu_1)\pi(1, 2, 0, 0) =\lambda_2\pi(1, 1, 0, 0) +\lambda_1\pi(0, 2, 0, 0)
(\lambda_3 +\lambda_1 +\lambda_2+2\mu_1)\pi(2, 0, 0, 0) =\mu_3\pi(2, 0, 1, 0)+3\mu_1\pi(3, 0, 0, 0) +\mu_2\pi(2, 1, 0, 0) +\lambda_1\pi(1, 0, 0, 0)
(\mu_2 +\lambda_1+2\mu_1)\pi(2, 1, 0, 0) =\lambda_2\pi(2, 0, 0, 0)+3\mu_1\pi(3, 1, 0, 0) +\lambda_1\pi(1, 1, 0, 0)
(\lambda_1 +\lambda_2+3\mu_1)\pi(3, 0, 0, 0) = 4\mu_1\pi(4, 0, 0, 0) +\mu_2\pi(3, 1, 0, 0) +\lambda_1\pi(2, 0, 0, 0)
(\mu_2+3\mu_1)\pi(3, 1, 0, 0) =\lambda_2\pi(3, 0, 0, 0) +\lambda_1\pi(2, 1, 0, 0)
(\lambda_1+4\mu_1)\pi(4, 0, 0, 0) = 5\mu_1\pi(5, 0, 0, 0) +\lambda_1\pi(3, 0, 0, 0)
5\mu_1\pi(5, 0, 0, 0) =\lambda_1\pi(4, 0, 0, 0)
\pi(2, 0, 1, 0) + \pi(1, 0, 1, 0) + \pi(0, 0, 1, 0) + \pi(0, 1, 1, 0) + \pi(0, 0, 0, 1) + \pi(0, 0, 0, 0) + \pi(0, 1, 0, 0) + \pi(0, 2, 0, 0) + \pi(1, 0, 0, 1) + \pi(1, 0, 0, 0) + \pi(1, 1, 0, 0) + \pi(1, 2, 0, 0) + \pi(2, 0, 0, 0) + \pi(2, 1, 0, 0) + \pi(3, 0, 0, 0) + \pi(3, 1, 0, 0) + \pi(4, 0, 0, 0) + \pi(5, 0, 0, 0) = 1
\lambda_1 = 24
\lambda_2 = 0.504
\lambda_3 = 0.144,
\lambda_4 = 0.072
\mu_1 = 0.167
\mu_2 = 0.05
\mu_3 = 0.05
\mu_4 = 0.05
